hinata_mikami/raw_ptr_tst/output/raw_ptr_tst/generated/generated_code_raw_ptr_tst.v
@@ -19,9 +19,69 @@ From rrstd.range.range.generated Require Export generated_specs_range.
 From rrstd.result.result.generated Require Export generated_specs_result.
 From rrstd.rr_internal.rr_internal.generated Require Export generated_specs_rr_internal.
 From rrstd.stdlib.stdlib.generated Require Export generated_specs_stdlib.
+Section Node_sls.
+  Context `{RRGS : !refinedrustGS Σ}.
+
+  Definition Node_sls  : struct_layout_spec :=
+    let Node_st  := UnitSynType in
+    mk_sls "Node" [
+    ("value", (IntSynType I32));
+    ("next", PtrSynType)] StructReprRust.
+  Definition Node_st  : syn_type := Node_sls .
+End Node_sls.
+
 Section code.
 Context `{RRGS : !refinedrustGS Σ}.
 Open Scope printing_sugar.
+
+Program Definition Node_id_Node_def  : function :=
+  {|
+     f_args := [
+      ("p", void* : layout)
+     ];
+     f_code :=
+      <[
+     "_bb0" :=
+      local_live{ PtrSynType } "__0";
+      "__0" <-{ PtrOp } copy{ PtrOp } ("p");
+      return (move{ PtrOp } ("__0"))
+     ]>%E $
+      ∅;
+     f_init := "_bb0";
+    |}.
+Next Obligation.
+  solve_fn_vars_nodup.
+Qed.
+
+
+
+
+Program Definition Node_set_next_def  : function :=
+  {|
+     f_args := [
+      ("node", void* : layout);
+     ("next", void* : layout)
+     ];
+     f_code :=
+      <[
+     "_bb0" :=
+      local_live{ UnitSynType } "__0";
+      local_live{ PtrSynType } "__3";
+      "__3" <-{ PtrOp } copy{ PtrOp } ("next");
+      (!{ PtrOp } ( "node" )) at{ Node_sls } "next" <-{ PtrOp } move{ PtrOp } ("__3");
+      local_dead "__3";
+      "__0" <-{ StructOp unit_sl [] } zst_val;
+      return (move{ StructOp unit_sl [] } ("__0"))
+     ]>%E $
+      ∅;
+     f_init := "_bb0";
+    |}.
+Next Obligation.
+  solve_fn_vars_nodup.
+Qed.
+
+
+
 
 Program Definition id_def  : function :=
   {|
@@ -46,28 +106,6 @@ Qed.
 
 
 Program Definition id_Cell_def  : function :=
-  {|
-     f_args := [
-      ("p", void* : layout)
-     ];
-     f_code :=
-      <[
-     "_bb0" :=
-      local_live{ PtrSynType } "__0";
-      "__0" <-{ PtrOp } copy{ PtrOp } ("p");
-      return (move{ PtrOp } ("__0"))
-     ]>%E $
-      ∅;
-     f_init := "_bb0";
-    |}.
-Next Obligation.
-  solve_fn_vars_nodup.
-Qed.
-
-
-
-
-Program Definition id_Node_def  : function :=
   {|
      f_args := [
       ("p", void* : layout)
